% !TEX TS-program = pdflatex
% !TEX encoding = UTF-8 Unicode

% This is a simple template for a LaTeX document using the "article" class.
% See "book", "report", "letter" for other types of document.

\documentclass[11pt]{article} % use larger type; default would be 10pt

\usepackage[utf8]{inputenc} % set input encoding (not needed with XeLaTeX)

%%% Examples of Article customizations
% These packages are optional, depending whether you want the features they provide.
% See the LaTeX Companion or other references for full information.

%%% PAGE DIMENSIONS
\usepackage{geometry} % to change the page dimensions
\geometry{a4paper} % or letterpaper (US) or a5paper or....
\geometry{margin=1in} % for example, change the margins to 2 inches all round
% \geometry{landscape} % set up the page for landscape
%   read geometry.pdf for detailed page layout information

\usepackage{graphicx} % support the \includegraphics command and options

% \usepackage[parfill]{parskip} % Activate to begin paragraphs with an empty line rather than an indent
\usepackage{amssymb}
\usepackage{amsmath}
%%% PACKAGES
\usepackage{booktabs} % for much better looking tables
\usepackage{array} % for better arrays (eg matrices) in maths
\usepackage{paralist} % very flexible & customisable lists (eg. enumerate/itemize, etc.)
\usepackage{verbatim} % adds environment for commenting out blocks of text & for better verbatim
\usepackage{subfig} % make it possible to include more than one captioned figure/table in a single float
% These packages are all incorporated in the memoir class to one degree or another...

%%% HEADERS & FOOTERS
\usepackage{fancyhdr} % This should be set AFTER setting up the page geometry
\pagestyle{fancy} % options: empty , plain , fancy
\renewcommand{\headrulewidth}{0pt} % customise the layout...
\lhead{}\chead{}\rhead{}
\lfoot{}\cfoot{\thepage}\rfoot{}

%%% SECTION TITLE APPEARANCE
\usepackage{sectsty}
\allsectionsfont{\sffamily\mdseries\upshape} % (See the fntguide.pdf for font help)
% (This matches ConTeXt defaults)

%%% ToC (table of contents) APPEARANCE
\usepackage[nottoc,notlof,notlot]{tocbibind} % Put the bibliography in the ToC
\usepackage[titles,subfigure]{tocloft} % Alter the style of the Table of Contents

\renewcommand{\cftsecfont}{\rmfamily\mdseries\upshape}
\renewcommand{\cftsecpagefont}{\rmfamily\mdseries\upshape} % No bold!
\DeclareMathOperator*{\argmax}{arg\,max}
\DeclareMathOperator*{\argmin}{arg\,min}

\newcount\colveccount
\newcommand*\colvec[1]{
        \global\colveccount#1
        \begin{pmatrix}
        \colvecnext
}
\def\colvecnext#1{
        #1
        \global\advance\colveccount-1
        \ifnum\colveccount>0
                \\
                \expandafter\colvecnext
        \else
                \end{pmatrix}
        \fi
}

\newcommand{\norm}[1]{\left\lVert#1\right\rVert}

\title{Econometrics HW4}
\author{Michael B. Nattinger\footnote{I worked on this assignment with my study group: Alex von Hafften, Andrew Smith, and Ryan Mather. I have also discussed problem(s) with Emily Case, Sarah Bass, and Danny Edgel.}}

\begin{document}
\maketitle

\section{Question 1}
\subsection{Show that $\bar{X}_{n+1} = (n\bar{X}_n + X_{n+1})/(n+1).$}
\begin{align*}
\bar{X}_{n+1} &= \frac{1}{n+1}\sum_{i=1}^{n+1} X_i = \frac{1}{n+1}\left(\left(\sum_{i=1}^n X_i\right) +X_{n+1}\right) \\ 
&=  \frac{1}{n+1}\left(n\bar{X}_n +X_{n+1}\right).
\end{align*}
\subsection{Show that $s_{n+1}^2 = ((n-1)s_n^2 + (n/(n+1))(X_{n+1} - \bar{X}_n)^2)/n.$}
%\begin{align*}
%s_{n+1}^2 &= \frac{1}{n}\sum_{i=1}^{n+1}(X_i - \bar{X}_{n+1})^2 =  \frac{1}{n}\sum_{i=1}^{n+1}(X_i - \frac{1}{n+1}\left(n\bar{X}_n +X_{n+1}\right))^2 \\
%&=\frac{1}{n}\left(\left(\sum_{i=1}^{n}(X_i - \frac{1}{n+1}\left(n\bar{X}_n +X_{n+1}\right))^2\right) + (X_{n+1} - \frac{1}{n+1}(n\bar{X}_n + X_{n+1}) )^2\right) \\
%&=\frac{1}{n}\left(\left(\sum_{i=1}^{n}(X_i - \frac{n}{n+1}\bar{X}_n -X_{n+1})^2\right) + (\frac{n}{n+1}(X_{n+1} - \bar{X}_n ) )^2\right) 
%\end{align*}
\begin{align*}
s_{n+1}^2 &= \frac{1}{n}\sum_{i=1}^{n+1}(X_i - \bar{X}_{n+1})^2 = \frac{1}{n}\sum_{i=1}^{n+1}(X_i - \bar{X}_{n} + \bar{X}_{n}+ \bar{X}_{n+1})^2\\
&= \frac{1}{n}\left( (n-1)\sum_{i=1}^{n+1}(X_i - \bar{X}_{n+1})^2 +n(\bar{X}_{n} - \bar{X}_{n+1}) + 2(\sum_{i=1}^n (X_j - \bar{X}_{n})(\bar{X}_{n} - \bar{X}_{n+1})) + (X_{n+1} - \bar{X}_{n+1})\right) \\
&= \frac{1}{n}\left( (n-1)\sum_{i=1}^{n+1}(X_i - \bar{X}_{n+1})^2 +n(\bar{X}_{n} - \bar{X}_{n+1})^2 + (X_{n+1} - \bar{X}_{n+1})^2\right) \\
&= \frac{1}{n}\left( (n-1)s_{n}^2 +n\bar{X}_{n}^2 - 2n\bar{X}_{n}\bar{X}_{n+1} +n \bar{X}_{n+1}^2 + X_{n+1}^2 - 2X_{n+1}\bar{X}_{n+1}+\bar{X}_{n+1}^2\right)\\
&= \frac{1}{n}\left( (n-1)s_{n}^2 + \frac{n}{n+1}(X_{n+1} - \bar{X}_{n})^2\right).
\end{align*}
\section{Question 2}
Define $\hat{\mu}_k:= \frac{1}{n}\sum_{i=1}^{n}X_i^k.$ We will show that this is unbiased.
\begin{align*}
E[\hat{\mu}_k] &= E\left[\frac{1}{n}\sum_{i=1}^{n}X_i^k\right] = \frac{1}{n}\sum_{i=1}^nE[X_i^k]\\
 &=\frac{1}{n}\sum_{i=1}^n\mu_k \\
&= \mu_k.
\end{align*}
Thus, $\hat{\mu}_k$ is an unbiased estimator for $\mu_k$.
\section{Question 3}
Define $\hat{M}_k:= \frac{1}{n}\sum_{i=1}^n (X_i - \bar{X})^k$. This estimator is biased, which can be seen from the fact that $\hat{M}_2 = \hat{\sigma}^2 \neq s_{n}^2$, so $\hat{M}_2$ is not an unbiased estimator for $M_2 = \sigma^2$. There exists no general formula for an unbiased estimator of $M_k.$
\section{Question 4}
%\begin{align*}
%E[(\hat{\mu}_k - \mu)^2] = E\left[\left(  \frac{1}{n}\sum_{i=1}^n (X_i - \bar{X})^k - \mu\right)^2\right]
%\end{align*}
%other way?
\begin{align*}
E[(\hat{\mu}_k - E[\hat{\mu}_k])^2] &=  E\left[\left( \frac{1}{n}\sum_{i=1}^{n}X_i^k\right)^2\right] - E\left[\frac{1}{n}\sum_{i=1}^{n}X_i^k\right]^2 \\
&= \frac{1}{n^2}E\left[\left(\sum_{i=1}^{n}X_i^k\right)^2\right] - \mu_k^2 \\
&= \frac{1}{n^2}E\left[\left(\sum_{i=1}^{n}X_i^{2k}\right)+\sum_{1\leq i<j\leq n}X_i^k X_j^k\right] - \mu_k^2\\
&= \frac{1}{n^2}\left(\left(\sum_{i=1}^{n}E(X_i^{2k})\right) + \left(\sum_{1\leq i<j\leq n}E(X_i^k X_j^k)\right) -  \mu_k^2\right) \\
&= \frac{1}{n^2}\left(n\mu_{2k} + \left(\sum_{1\leq i<j\leq n}E(X_i^k)E(X_j^k)\right) -  \mu_k^2\right) \\
&= \frac{1}{n^2}\left(n\mu_{2k} + \left(\frac{n!}{2(n-2)!}\right)\mu_k^2 -  \mu_k^2\right)  = \frac{1}{n}\mu_{2k} + \left(\frac{n-1}{2n} - \frac{1}{n}\right)\mu_k^2\\
&= \frac{1}{n}\mu_{2k} + \left(\frac{n-3}{2n}\right)\mu_k^2\\
\Rightarrow Var(\hat{\mu}_k) &= \frac{1}{n}\mu_{2k} + \left(\frac{n-3}{2n}\right)\mu_k^2
\end{align*}
\section{Question 5}
Note that $f(x) = x^2$ is convex. By Jensen's inequality,
\begin{align*}
E[s_n]^2 \leq E[s_n^2] = \sigma^2,
\end{align*}
so $E[s_n]\leq \sigma$ as both are nonnegative.
\section{Question 6}
\begin{align*}
\hat{\sigma}^2 &= \frac{1}{n}\sum_{i=1}^{n}(X_i - \bar{X}_{n})^2 = \frac{1}{n}\sum_{i=1}^{n}(X_i^2 -2X_i\bar{X}_{n} +  \bar{X}_{n}^2) \\
&= \frac{1}{n}\left(\sum_{i=1}^{n}X_i^2 -2\bar{X}_{n}\sum_{i=1}^nX_i +  \bar{X}_{n}^2\sum_{i=1}^n1\right) \\
&= \frac{1}{n}\left(\sum_{i=1}^{n}X_i^2 -2n\bar{X}_{n}^2 +  n\bar{X}_{n}^2\right) = \frac{1}{n}\left(\sum_{i=1}^{n}X_i^2 -n\bar{X}_{n}^2 \right) .\\
\frac{1}{n}\sum_{i=1}^{n}(X_i - \mu)^2- ( \bar{X}_{n} - \mu)^2 &= \frac{1}{n}\sum_{i=1}^{n}X_i^2 - 2X_i\mu + \mu^2-  \bar{X}_{n}^2 + 2\mu\bar{X}_{n}- \mu^2\\
&= \frac{1}{n}\sum_{i=1}^{n}X_i^2  -  \bar{X}_{n}^2 + 2\mu(\bar{X}_{n} - X_i) \\
&= \frac{1}{n}\left(\sum_{i=1}^{n}X_i^2  -  \bar{X}_{n}^2\sum_{i=1}^{n}(1) +\sum_{i=1}^{n}2\mu(\bar{X}_{n} - X_i) \right)\\
&= \frac{1}{n}\left(\sum_{i=1}^{n}X_i^2 -n\bar{X}_{n}^2 \right) = \hat{\sigma}^2.
\end{align*}
\section{Question 7}
%\begin{align*}
%Cov(\hat{\sigma}^2,\bar{X}_n) &= E[\hat{\sigma}^2\bar{X}_n] - E[\hat{\sigma}^2]E[\bar{X}_n] \\
%&=  E\left[\left(\frac{1}{n}\sum_{i=1}^{n}(X_i - \mu)^2- ( \bar{X}_{n} - \mu)^2\right)\left( \frac{1}{n}\sum_{i=1}^{n}X_i\right)\right] - \frac{n-1}{n}\sigma^2\mu \\
%&= \frac{1}{n^2} E\left[\left(\sum_{i=1}^{n}(X_i - \mu)^2- ( \bar{X}_{n} - \mu)^2\right)\left(\sum_{i=1}^{n}X_i\right)\right] - \frac{n-1}{n}\sigma^2\mu \\
%&= \frac{1}{n^2} E\left[\sum_{i=1}^{n}\sum_{j=1}^{n}X_j(X_i - \mu)^2- X_j( \bar{X}_{n} - \mu)^2\right] - \frac{n-1}{n}\sigma^2\mu \\
%&= \frac{1}{n^2} E\left[\sum_{i=1}^{n}\sum_{j=1}^{n}X_j(X_i - \mu)^2\right]-\frac{1}{n^2}E\left[ \sum_{i=1}^{n}\sum_{j=1}^{n}X_j( \bar{X}_{n} - \mu)^2\right] - \frac{n-1}{n}\sigma^2\mu \\
%&= \frac{1}{n^2} E\left[\sum_{i \neq j}^{n}X_j(X_i - \mu)^2\right]+\frac{1}{n^2} E\left[\sum_{i=1}^{n}X_i(X_i - \mu)^2\right]-\frac{1}{n}E\left[\sum_{j=1}^{n}X_j( \bar{X}_{n} - \mu)^2\right] - \frac{n-1}{n}\sigma^2\mu \\
%&= \frac{1}{n^2} E\left[\sum_{i \neq j}^{n}X_j(X_i - \mu)^2\right]+\frac{1}{n^2} E\left[\sum_{i=1}^{n}X_i(X_i - \mu)^2\right]  - \frac{1}{n}E\left[\bar{X}_n(\bar{X}_n - \mu)^2 \right]- \frac{n-1}{n}\sigma^2\mu \\
%&= \frac{1}{n^2} \sum_{i \neq j}EX_jE(X_i - \mu)^2+\frac{1}{n^2} \sum_{i=1}^{n}E\left[X_i(X_i - \mu)^2\right]  - \frac{1}{n}E\left[\bar{X}_n(\bar{X}_n - \mu)^2 \right]- \frac{n-1}{n}\sigma^2\mu \\
%&= \frac{n!}{2n^2(n-2)!} \mu\sigma^2+\frac{1}{n^2} \sum_{i=1}^{n}E\left[X_i(X_i - \mu)^2\right]  - \frac{1}{n}E\left[\bar{X}_n(\bar{X}_n - \mu)^2 \right]- \frac{n-1}{n}\sigma^2\mu \\
%&= \frac{n-1}{2n} \mu\sigma^2+\frac{1}{n^2} \sum_{i=1}^{n}E\left[X_i(X_i - \mu)^2\right]  - \frac{1}{n}E\left[\bar{X}_n(\bar{X}_n - \mu)^2 \right]- \frac{n-1}{n}\sigma^2\mu 
%\end{align*}
\begin{align*}
Cov(\hat{\sigma}^2,\bar{X}_n) &= Cov\left(\frac{1}{n}\sum_{i=1}^{n}(X_i - \mu)^2- ( \bar{X}_{n} - \mu)^2,\frac{1}{n}\sum_{i=1}^{n}X_i\right) \\
&= \frac{1}{n^2}Cov\left(\sum_{i=1}^{n}(X_i - \mu)^2- ( \bar{X}_{n} - \mu)^2,\sum_{i=1}^{n}X_i\right) \\
&= \frac{1}{n^2}\sum_{i=1}^{n}Cov\left(\sum_{j=1}^{n}(X_j - \mu)^2- ( \bar{X}_{n} - \mu)^2,X_i\right) %&= \frac{1}{n^2}\sum_{i=1}^{n}\left(Cov\left(\sum_{j=1}^{n}(X_j - \mu)^2- ( \bar{X}_{n} - \mu)^2,X_i\right) + Cov\left( \right) \right)
\end{align*}
This question is far from solved.
\section{Question 8}
\subsection{Find $E[\bar{X}_n]$}
\begin{align*}
E[\bar{X}_n] &= E\left[\frac{1}{n} \sum_{i=1}^{n} X_i \right] = \frac{1}{n}\sum_{i=1}^{n} E\left[X_i \right] \\
&= \frac{1}{n}\sum_{i=1}^{n} \mu_i.
\end{align*}
\subsection{Find $Var(\bar{X}_n)$.}
\begin{align*}
Var(\bar{X}_n) &= E[\bar{X}_n^2] - (E\bar{X}_n)^2 = E\left[\left(\frac{1}{n} \sum_{i=1}^{n} X_i\right)^2\right]  - \left(\frac{1}{n}\sum_{i=1}^{n}  \mu_i\right)^2 \\
&= \frac{1}{n^2}E\left[\left( \sum_{i=1}^{n} X_i\right)^2\right]  - \left(\frac{1}{n}\sum_{i=1}^{n}  \mu_i\right)^2 \\
&= \frac{1}{n^2}E\left[\left( \sum_{i=1}^{n} X_i^2\right) + 2\left(\sum_{1\leq i<j \leq n} X_iX_j\right)  \right]  - \left(\frac{1}{n}\sum_{i=1}^{n}  \mu_i\right)^2\\
&= \frac{1}{n^2}\left( \sum_{i=1}^{n} EX_i^2\right) + \frac{2}{n^2}\left(\sum_{1\leq i<j \leq n} EX_iX_j\right)    - \left(\frac{1}{n}\sum_{i=1}^{n}  \mu_i\right)^2\\
&= \frac{1}{n^2}\left( \sum_{i=1}^{n} \sigma_i^2 + \mu_i^2\right) + \frac{2}{n^2}\left(\sum_{1\leq i<j \leq n} \mu_i \mu_j\right)    - \left(\frac{1}{n}\sum_{i=1}^{n}  \mu_i\right)^2.
\end{align*}
\section{Question 9}
\begin{align*}
E[Q] &= E\left[ \sum_{i=1}^r X_i^2 \right] = \sum_{i=1}^n E\left[ X_i^2 \right]  \\
&=  \sum_{i=1}^r \mu_X^2 + \sigma_X^2 = \sum_{i=1}^n 0^2 + 1^2\\
&=  r.
\end{align*}
\begin{align*}
Var(Q) &= E[Q^2] - E[Q]^2 = E\left[\left(\sum_{i=1}^r X_i^2 \right)^2\right] - r^2\\
&= \sum_{i=1}^r E\left[X_i^4\right] + 2\sum_{1\leq i < j \leq r}E\left[ X_i^2X_j^2\right] -r^2 \\
&= \sum_{i=1}^r 3 + 2\sum_{1\leq i < j \leq r}(1)(1) -r^2 \\
&= 3r + 2\left( \frac{r!}{2(r-2)!}\right) -r^2 = 3r + r(r-1) -r^2 \\
&= 2r.
\end{align*}
Note: we calculated $E[x^4]=3$ for a standard normal in the previous problem set.
\section{Question 10}
We will first show that a sum of independent normal random variables is normal. Let $Z_i\sim N(\mu_i,\sigma_i^2) \forall i \in [1,\dots,n]$ for some $n \in \mathbb{N}.$ Then the MGF of $Z_i$ is $M_{Z_i}(t) = exp(\mu_i t + \frac{\sigma_i^2t^2}{2})$.\footnote{$M_{Z_i}(t) = \int_{-\infty}^{\infty}exp(xt)\frac{1}{\sqrt{2\pi\sigma_i^2}}exp(-(x-\mu_i)^2/(2\sigma_i^2))dx.$ Define $z = (x-\mu_i)/\sigma_i.$ Then $M_{Z_i}(t) =exp(\mu_it)\int_{-\infty}^{\infty}exp(z\sigma t)\frac{1}{\sqrt{2\pi\sigma_i^2}} exp(-z^2/2) (dx/dz)dz = exp(\mu_it)\int_{-\infty}^{\infty}exp(z\sigma t)\frac{1}{\sqrt{2\pi}} exp(-z^2/2)dz  = exp(\mu_it)exp(\sigma_i^2t^2/2) = exp(\mu_it + \frac{\sigma_i^2t^2}{2}).$} Then,\footnote{$M_{\sum_{i=1}^n{Z_i}}(t) = E[exp(\sum_{i=1}^n tZ_i)] = E[\prod_{i=1}^{n}exp(tZ_i)] = \prod_{i=1}^{n}E[exp(tZ_i)] = \prod_{i=1}^{n}M_{Z_i}(t)$}
\begin{align*}
M_{\sum_{i=1}^n{Z_i}}(t) = \prod_{i=1}^nM_{Z_i}(t) = exp\left( \sum_{i=1}^n \left(\mu_it + \frac{\sigma_i^2t}{2}\right)\right) = exp\left( \left(\sum_{i=1}^n \mu_i\right)t + \left( \sum_{i=1}^n \sigma_i^2\right)\frac{t^2}{2}\right).
\end{align*}
So $\sum_{i=1}^nZ_i$ is of the form of a normal random variable with mean $\sum_{i=1}^n\mu_i$ and variance $\sum_{i=1}^n\sigma_i^2$.
\subsection{Find $E[\bar{X}_n - \bar{Y}_n]$}
From the above, $\bar{X}_n,\bar{Y}_n$ are of the form of normal variables with means $\mu_X,\mu_Y$ and variances $\frac{1}{n_1}\sigma_X^2,\frac{1}{n_2}\sigma_Y^2$. Then, $\bar{X}_n-\bar{Y}_n$ is also normal with mean $\mu_X-\mu_Y$.
\subsection{Find $Var[\bar{X}_n - \bar{Y}_n]$}
From the above, $\bar{X}_n-\bar{Y}_n$ is normal with variance $\frac{1}{n_1}\sigma_X^2 + \frac{1}{n_2}\sigma_Y^2$.
\subsection{Find the distribution of $\bar{X}_n - \bar{Y}_n$}
From the above, $\bar{X}_n - \bar{Y}_n$ is of the form of a normal random variable with mean $\mu_X-\mu_Y$ and variance $\frac{1}{n_1}\sigma_X^2 + \frac{1}{n_2}\sigma_Y^2$.
\end{document}
